rocq-skylabs-cpp2v/tests/floating_casts_extra.t/test.v
@@ -1,0 +1,7 @@
+Require Import skylabs.prelude.base.
+Require Import skylabs.lang.cpp.syntax.supported.
+Require test.test_cpp.
+
+Example generated_float_casts_supported :
+  supported.check.translation_unit test_cpp.module = [] :=
+  ltac:(vm_compute; reflexivity).
